Updates

high2/Zeta.High.Blum.fst
@@ -1,6 +1,7 @@
 module Zeta.High.Blum
 
 open Zeta.High.Thread
+open Zeta.SeqIdx
 
 let eac_state_transition_snoc
   (#app #n:_)
@@ -178,45 +179,95 @@ let eac_evictedm_addb_diff_elem
     lemma_evict_before_add2 ep itsl (i+1) be';
     be'
 
+open Zeta.High.Verifier
+
+let is_blum_evict_refs_key (#app:_) (k: base_key) (e: vlog_entry app)
+  = let open Zeta.GenericVerifier in
+    e `refs_key` k &&
+    is_blum_evict e
+
+(* switch order of params ... *)
+let refs_key (#app:_) (k: base_key) (e: vlog_entry app)
+  = e `refs_key` k
+
+let last_evict_props
+  (#app #n:_)
+  (k: base_key)
+  (itsl: eac_log app n {EACEvictedBlum? (eac_state_of_key k itsl)})
+  : Lemma (ensures (let l = i_seq itsl in
+                    let EACEvictedBlum gke ve te tide = eac_state_of_key k itsl in
+                    exists_elems_with_prop (is_blum_evict_refs_key k) l /\
+                    (let j = last_idx (is_blum_evict_refs_key k) l in
+                     let MHDom (gk,v) t tid  = blum_evict_elem itsl j in
+                     gk = gke /\ v = ve /\ t = te /\ tid = tide /\
+                     j = last_idx (refs_key k) l)))
+  = admit()
+
+module S = FStar.Seq
+
+let next_add
+  (#app #n:_)
+  (k: base_key)
+  (itsl: eac_log app n {EACEvictedBlum? (eac_state_of_key k itsl)})
+  (i: seq_index itsl {let l = i_seq itsl in
+                      is_blum_evict_refs_key k (index itsl i) /\
+                      i <> last_idx (refs_key k) l})
+  : j:seq_index itsl{is_blum_add itsl j /\
+                     blum_add_elem itsl j = blum_evict_elem itsl i}
+  = admit()
+
+module GV = Zeta.GenericVerifier
+
+#push-options "--z3rlimit_factor 3"
+
 let eac_evictedb_addb_diff_elem
   (#app #n:_)
-  (itsl: its_log app n)
-  (i: seq_index itsl{let itsli = prefix itsl i in
-                     let itsli' = prefix itsl (i + 1) in
-                     is_blum_add itsl i /\
-                     is_eac itsli /\
-                     not (is_eac itsli') /\
-                     (let e = index itsl i in
-                      let k = add_slot e in
-                      let es = eac_state_of_key k itsli in
-                      EACEvictedBlum? es)})
-  : (be':ms_hashfn_dom app{let ep = be'.t.e in
-                           let as = add_set ep itsl in
-                           let es = evict_set ep itsl in
-                           let be = blum_add_elem itsl i in
+  (il: neac_log app n {let i = eac_boundary il in
+                         let k = eac_fail_key il in
+                         Zeta.Generic.TSLog.clock_sorted il /\
+                         is_blum_add il i /\
+                         EACEvictedBlum? (eac_state_of_key_pre k il i)})
+  : (be':ms_hashfn_dom app{let i = eac_boundary il in
+                           let ep = be'.t.e in
+                           let as = add_set ep il in
+                           let es = evict_set ep il in
+                           let be = blum_add_elem il i in
                            mem be' as > mem be' es /\
                            be.t.e = ep})
-  = let itsli = prefix itsl i in
-    let itsli' = prefix itsl (i+1) in
-    let e = index itsl i in
-    let k = add_slot e in
-    let be = blum_add_elem itsl i in
+  = let i = eac_boundary il in
+    let itsli = prefix il i in
+    let k = eac_fail_key il in
+    let EACEvictedBlum gk_e v_e t_e tid_e = eac_state_of_key_pre k il i in
+    eac_state_transition k il i;
+    lemma_cur_thread_state_extend il i;
+
+    let be = blum_add_elem il i in
+    let gk,v = be.r in
     let ep = be.t.e in
-    let gk,_ = be.r in
 
-    //assert(to_base_key gk = k);
-    evict_add_count_rel ep gk itsli;
-    admit()
+    // otherwise we would not have an EAC failure at i
+    assert(gk <> gk_e || v <> v_e || be.t <> t_e || be.tid <> tid_e);
 
-(* when the eac store is evicted, there exists a previous evict *)
-let previous_evict_of_eac_evicted
-  (#app #n:_)
-  (itsl: eac_log app n)
-  (k: base_key {EACEvictedBlum? (eac_state_of_key k itsl)})
-  : i:seq_index itsl{is_blum_evict itsl i /\
-                     (let be = blum_evict_elem itsl i in
-                      let EACEvictedBlum gk v t j = eac_state_of_key k itsl in
-                      let gk',v' = be.r in
-                      let open Zeta.MultiSetHashDomain in
-                      gk = gk' /\ v = v' /\ be.t = t /\ be.tid = j)}
-  = admit()
+    if evict_set ep il `contains` be then (
+      last_evict_props k itsli;
+      let j = last_idx (is_blum_evict_refs_key k) (i_seq itsli) in
+      let be' = blum_evict_elem il j in
+      assert(be' <> be);
+
+      let i' = evict_elem_idx il be in
+      let e = index il i' in
+      let be2 = blum_evict_elem il i' in
+      assert(GV.is_blum_evict e);
+      assert(is_blum_evict_refs_key k e);
+      lemma_evict_before_add il i;
+
+      assert(i' < i);
+
+      //last_idx_correct (is_blum_evict_refs_key k) (i_seq itsli) i';
+
+      admit()
+    )
+    else
+      be
+
+#pop-options
