high2/Zeta.High.Blum.fsti
@@ -50,31 +50,16 @@ val eac_evictedm_addb_diff_elem
 
 val eac_evictedb_addb_diff_elem
   (#app #n:_)
-  (itsl: its_log app n)
-  (i: seq_index itsl{let itsli = prefix itsl i in
-                     let itsli' = prefix itsl (i + 1) in
-                     is_blum_add itsl i /\
-                     is_eac itsli /\
-                     not (is_eac itsli') /\
-                     (let e = index itsl i in
-                      let k = add_slot e in
-                      let es = eac_state_of_key k itsli in
-                      EACEvictedBlum? es)})
-  : (be':ms_hashfn_dom app{let ep = be'.t.e in
+  (itsl: neac_log app n {let i = eac_boundary itsl in
+                         let k = eac_fail_key itsl in
+                         Zeta.Generic.TSLog.clock_sorted itsl /\
+                         is_blum_add itsl i /\
+                         EACEvictedBlum? (eac_state_of_key_pre k itsl i)})
+  : (be':ms_hashfn_dom app{let i = eac_boundary itsl in
+                           let ep = be'.t.e in
                            let as = add_set ep itsl in
                            let es = evict_set ep itsl in
                            let be = blum_add_elem itsl i in
                            mem be' as > mem be' es /\
                            be.t.e = ep})
 
-(* when the eac store is evicted, there exists a previous evict *)
-val previous_evict_of_eac_evicted
-  (#app #n:_)
-  (itsl: eac_log app n)
-  (k: base_key {EACEvictedBlum? (eac_state_of_key k itsl)})
-  : i:seq_index itsl{is_blum_evict itsl i /\
-                     (let be = blum_evict_elem itsl i in
-                      let EACEvictedBlum gk v t j = eac_state_of_key k itsl in
-                      let gk',v' = be.r in
-                      let open Zeta.MultiSetHashDomain in
-                      gk = gk' /\ v = v' /\ be.t = t /\ be.tid = j)}
